store/client_proofs/close.v
@@ -30,27 +30,35 @@ Variable N : namespace.
 Lemma wp_client_close c kI kR cs :
   channel c -∗
   store_ctx N -∗
-  {{{ client_connected kI kR cs }}}
+  {{{ db_connected kI kR cs }}}
     Client.close N c (repr cs)
   {{{ RET #(); db_disconnected kI kR }}}.
 Proof.
 iIntros "#chan_c (_ & _ & _ & _ & _ & _ & _ & _ & #close & #ack & _)".
 iIntros "!> %Φ client post".
-iDestruct "client"
-  as "(%n & %beginning & <- & <- & %e_rl & #conn & rel & ts & client)".
+iDestruct "client" as "(%n & %beginning & client & conn)".
+iPoseProof (client_connected_wf_conn_state with "conn") as "#?".
 wp_lam; wp_pures.
-wp_apply (wp_connection_timestamp with "ts"). iIntros "ts".
+wp_apply (wp_connection_timestamp_client with "conn"). iIntros "conn".
+iAssert (⌜cs_role cs = Init⌝)%I as "%e_rl".
+{ by iDestruct "conn" as "(? & ? & ? & ?)". }
 wp_pures. wp_apply wp_tint. wp_pures.
-iMod (close_predI with "client") as "(client & #p_m1)" => //.
+iMod (close_predI with "client conn") as "(client & #p_m1)" => //.
 wp_bind (Connection.send _ _ _ _).
-wp_apply (wp_connection_send with "[//] close [] [] conn") => //.
+wp_apply (wp_connection_send with "[//] close [] [] [//]") => //.
 { by rewrite public_TInt. }
 { by iIntros "!> _". }
 iIntros "_". wp_pures.
-iCombine "client post" as "I". iRevert "ts rel I".
+iDestruct "client" as "(client & conn)".
+iDestruct "conn" as "(% & % & #? & ts & rel & end & #ending & #conn)".
+iCombine "client end post" as "I". iRevert "ts rel I".
+have ->: si_init_share cs = cs_share cs.
+{ by rewrite /cs_share e_rl. }
 iApply wp_connection_recv => //.
-iIntros "!> %m ts rel (client & post) #m_m #inv'".
-iMod (ack_close_predE with "client inv'") as "client" => //.
+iIntros "!> %m ts rel (client & end & post) #m_m #inv'".
+iMod (ack_close_predE with "[ts rel end client] inv'")
+  as "[ts client]" => //.
+{ iFrame. rewrite /cs_share e_rl /=. iFrame. eauto. }
 wp_pures. wp_apply (wp_connection_close with "ts").
 iIntros "_". wp_pures.
 iRight. iModIntro. iExists _. iSplit; eauto.
