store/client_proofs/create.v
@@ -32,27 +32,27 @@ Lemma wp_client_create c kI kR cs t1 t2 :
   store_ctx N -∗
   public t1 -∗
   public t2 -∗
-  {{{ client_connected kI kR cs ∗
+  {{{ db_connected kI kR cs ∗
       rem_free_at kI kR {[t1]} }}}
     Client.create N c (repr cs) t1 t2
   {{{ (b : bool), RET #b;
-      client_connected kI kR cs ∗
+      db_connected kI kR cs ∗
       rem_mapsto kI kR t1 t2 }}}.
 Proof.
 iIntros "#chan_c (_ & _ & _ & _ & _ & _ & #create & #ack & _) #p_t1 #p_t2".
 iIntros "!> %Φ [client free] post".
-iDestruct "client"
-  as "(%n & %beginning & <- & <- & %e_rl & #conn & rel & ts & client)".
+iDestruct "client" as "(%n & %beginning & client & conn)".
+iPoseProof (client_connected_wf_conn_state with "conn") as "#?".
 rewrite /Client.create. wp_pures.
-iMod (@rem_mapsto_alloc _ _ _ _ _ t1 t2 with "client free")
+iMod (@rem_mapsto_alloc _ _ _ _ _ _ t1 t2 with "client free")
   as "(client & mapsto & _ & #created)".
 { by rewrite elem_of_singleton. }
 wp_bind (Connection.timestamp _).
-iApply (wp_connection_timestamp with "ts").
-iIntros "!> ts". wp_pures.
+iApply (wp_connection_timestamp_client with "conn").
+iIntros "!> conn". wp_pures.
 wp_bind (Connection.tick _).
-iApply (wp_connection_tick with "ts"). iIntros "!> ts".
-iDestruct (create_predI with "client p_t1 p_t2 created")
+iApply (wp_connection_tick_client with "conn"). iIntros "!> conn".
+iDestruct (create_predI with "conn p_t1 p_t2 created")
   as "#p_m1".
 wp_list. wp_bind (tint _). iApply wp_tint. wp_list. wp_term_of_list. wp_pures.
 wp_bind (Connection.send _ _ _ _).
@@ -60,9 +60,9 @@ iApply (wp_connection_send with "[//] create [] []") => //.
 { by rewrite public_of_list /= public_TInt; eauto. }
 { by iIntros "!> _". }
 iIntros "!> _". wp_pures.
-iCombine "client mapsto post" as "I". iRevert "ts rel I".
-iApply wp_connection_recv => //.
-iIntros "!> %m ts rel (client & mapsto & post) #m_m #inv'".
+iCombine "client mapsto post" as "I". iRevert "conn I".
+iApply wp_connection_recv_client => //.
+iIntros "!> %m conn (client & mapsto & post) #m_m #inv'".
 wp_pures. wp_list_of_term m; wp_pures; last by iLeft; iFrame.
 wp_list_match => [ts' k' v' b -> {m}|_] /=; wp_pures; last by iLeft; iFrame.
 wp_bind (tint _). iApply wp_tint.
