store/client_proofs/load.v
@@ -32,38 +32,39 @@ Lemma wp_client_load c kI kR cs t1 t2 :
   channel c -∗
   store_ctx N -∗
   public t1 -∗
-  {{{ client_connected kI kR cs ∗
+  {{{ db_connected kI kR cs ∗
       rem_mapsto kI kR t1 t2 }}}
     Client.load N c (repr cs) t1
   {{{ t2', RET (repr t2');
-      client_connected kI kR cs ∗
+      db_connected kI kR cs ∗
       rem_mapsto kI kR t1 t2 ∗
       public t2' ∗
       session_failed_or cs ⌜t2' = t2⌝ }}}.
 Proof.
 iIntros "#chan_c #ctx #p_t1 !> %Φ [client mapsto] post".
+iDestruct "client" as "(%n & %beginning & client & conn)".
+iPoseProof (client_connected_wf_conn_state with "conn") as "#?".
 iDestruct "ctx" as "(_ & _ & _ & _ & load & ack_load & _)".
-iDestruct "client"
-  as "(%n & %beginning & <- & <- & %e_rl & #conn & rel & ts & client)".
-rewrite /Client.load. wp_pures. wp_bind (Connection.timestamp _).
-iApply (wp_connection_timestamp with "ts"). iIntros "!> ts".
+rewrite /Client.load. wp_pures.
+wp_apply (wp_connection_timestamp_client with "conn"). iIntros "conn".
 wp_bind (tint _). iApply wp_tint.
-wp_pures. wp_apply (wp_connection_tick with "ts"). iIntros "ts".
+iMod (load_predI _ _ _ _ _ t1 with "client conn")
+  as "(client & conn & #load_at & #?)".
+wp_pures. wp_apply (wp_connection_tick_client with "conn"). iIntros "conn".
 wp_pures. wp_list. wp_term_of_list.
-iMod (load_predI _ _ _ t1 with "client") as "(client & #load_at & #?)".
 wp_bind (Connection.send _ _ _ _).
 iApply (wp_connection_send with "[//] load [] [#]") => //.
 { rewrite public_of_list /= public_TInt. by eauto. }
 { by iIntros "!> _". }
 iIntros "!> _". wp_pures.
-iCombine "client mapsto post" as "I". iRevert "ts rel I".
-iApply wp_connection_recv => //.
-iIntros "!> %ts ts rel (client & mapsto & post) #p_m #inv_m". wp_pures.
+iCombine "client mapsto post" as "I". iRevert "conn I".
+iApply wp_connection_recv_client => //.
+iIntros "!> %ts conn (client & mapsto & post) #p_m #inv_m". wp_pures.
 wp_list_of_term ts; wp_pures; last by iLeft; iFrame.
 wp_list_match => [n' t2' -> {ts}|_]; wp_pures; last by iLeft; iFrame.
 wp_eq_term e; last by wp_pures; iLeft; iFrame.
 subst n'. wp_pures.
-iPoseProof (ack_loadE with "client load_at mapsto p_m inv_m") as "#p_t2'".
+iPoseProof (ack_loadE with "client conn load_at mapsto p_m inv_m") as "#p_t2'".
 iRight. iModIntro. iExists _. iSplit => //.
 iApply "post".
 iFrame.
