store/client_proofs/store.v
@@ -32,45 +32,43 @@ Lemma wp_client_send_store c kI kR cs t1 t2 t2' :
   store_ctx N -∗
   public t1 -∗
   public t2' -∗ (* FIXME: t1 and t2' shouldn't have to be public already *)
-  {{{ client_connected kI kR cs ∗ rem_mapsto kI kR t1 t2 }}}
+  {{{ db_connected kI kR cs ∗ rem_mapsto kI kR t1 t2 }}}
     Client.send_store N c (repr cs) t1 t2'
-  {{{ RET #(); client_connected kI kR cs ∗ rem_mapsto kI kR t1 t2' }}}.
+  {{{ RET #(); db_connected kI kR cs ∗ rem_mapsto kI kR t1 t2' }}}.
 Proof.
 iIntros "#chan_c (_ & _ & #? & _) #p_t1 #p_t2' !> %Φ [client mapsto] post".
-iDestruct "client"
-  as "(%n & %beginning & <- & <- & %e_rl & #conn & rel & ts & client)".
+iDestruct "client" as "(%n & %beginning & client & conn)".
 iMod (rem_mapsto_store t2' with "client mapsto")
   as "(client & mapsto & #update)".
 wp_lam. wp_pures.
-wp_apply (wp_connection_timestamp with "ts"); iIntros "ts".
-wp_pures. wp_apply (wp_connection_tick with "ts"). iIntros "ts".
-iPoseProof (store_predI with "client update") as "#?".
+wp_apply (wp_connection_timestamp_client with "conn"); iIntros "conn".
+wp_pures. wp_apply (wp_connection_tick_client with "conn"). iIntros "conn".
+iPoseProof (store_predI with "[$] update") as "#?".
 wp_pures. wp_list. wp_bind (tint _). iApply wp_tint. wp_list.
 wp_term_of_list. wp_pures.
-iApply (wp_connection_send with "[//] [//] [] [#] conn") => //.
+iPoseProof (client_connected_wf_conn_state with "conn") as "#conn'".
+iApply (wp_connection_send with "[//] [//] [] [#] conn'") => //.
 { rewrite public_of_list /= public_TInt. by eauto. }
 { by iIntros "!> _". }
 iIntros "!> _".
-iApply ("post" with "[ts rel client mapsto]").
-by iFrame; eauto.
+iApply "post". by iFrame.
 Qed.
 
 Lemma wp_client_ack_store c kI kR cs :
   channel c -∗
   store_ctx N -∗
-  {{{ client_connected kI kR cs }}}
+  {{{ db_connected kI kR cs }}}
     Client.ack_store N c (repr cs)
-  {{{ RET #(); client_connected kI kR cs }}}.
+  {{{ RET #(); db_connected kI kR cs }}}.
 Proof.
 iIntros "#chan_c (_ & _ & _ & #? & _) !> %Φ client post".
-iDestruct "client"
-  as "(%n & %beginning & <- & <- & %e_rl & #conn & rel & ts & client)".
+iDestruct "client" as "(%n & %beginning & client & conn)".
 rewrite /Client.ack_store. wp_pures.
-wp_apply (wp_connection_timestamp with "ts"). iIntros "ts".
+wp_apply (wp_connection_timestamp_client with "conn"). iIntros "conn".
 wp_pures.
-iCombine "client post" as "I". iRevert "ts rel I".
-iApply wp_connection_recv => //.
-iIntros "!> %m ts rel (client & post) #m_m _".
+iCombine "client post" as "I". iRevert "conn I".
+iApply wp_connection_recv_client => //.
+iIntros "!> %m conn (client & post) #m_m _".
 wp_pures. wp_apply wp_tint.
 wp_eq_term e; wp_pures; last by iLeft; iFrame.
 iRight. iModIntro. iExists _. iSplit => //.
@@ -82,9 +80,9 @@ Lemma wp_client_store c kI kR cs t1 t2 t2' :
   store_ctx N -∗
   public t1 -∗
   public t2' -∗
-  {{{ client_connected kI kR cs ∗ rem_mapsto kI kR t1 t2 }}}
+  {{{ db_connected kI kR cs ∗ rem_mapsto kI kR t1 t2 }}}
     Client.store N c (repr cs) t1 t2'
-  {{{ RET #(); client_connected kI kR cs ∗ rem_mapsto kI kR t1 t2' }}}.
+  {{{ RET #(); db_connected kI kR cs ∗ rem_mapsto kI kR t1 t2' }}}.
 Proof.
 iIntros "#chan_c #ctx #p_t1 #p_t2 !> %Φ [client mapsto] post".
 rewrite /Client.store.
